WIP better types

dist/gcc-compatible/EverCrypt_Hash.c
@@ -54,7 +54,7 @@
 
 typedef uint8_t state_s_tags;
 
-typedef struct EverCrypt_Hash_state_s_s
+typedef struct state_s_s
 {
   state_s_tags tag;
   union {
@@ -75,11 +75,11 @@ typedef struct EverCrypt_Hash_state_s_s
   }
   ;
 }
-EverCrypt_Hash_state_s;
+state_s;
 
-static Spec_Hash_Definitions_hash_alg alg_of_state(EverCrypt_Hash_state_s *s)
+static Spec_Hash_Definitions_hash_alg alg_of_state(state_s *s)
 {
-  EverCrypt_Hash_state_s scrut = *s;
+  state_s scrut = *s;
   if (scrut.tag == MD5_s)
   {
     return Spec_Hash_Definitions_MD5;
@@ -143,69 +143,69 @@ static Spec_Hash_Definitions_hash_alg alg_of_state(EverCrypt_Hash_state_s *s)
   KRML_HOST_EXIT(255U);
 }
 
-static EverCrypt_Hash_state_s *create_in(Spec_Hash_Definitions_hash_alg a)
+static state_s *create_in(Spec_Hash_Definitions_hash_alg a)
 {
-  EverCrypt_Hash_state_s s;
+  state_s s;
   switch (a)
   {
     case Spec_Hash_Definitions_MD5:
       {
         uint32_t *buf = (uint32_t *)KRML_HOST_CALLOC(4U, sizeof (uint32_t));
-        s = ((EverCrypt_Hash_state_s){ .tag = MD5_s, { .case_MD5_s = buf } });
+        s = ((state_s){ .tag = MD5_s, { .case_MD5_s = buf } });
         break;
       }
     case Spec_Hash_Definitions_SHA1:
       {
         uint32_t *buf = (uint32_t *)KRML_HOST_CALLOC(5U, sizeof (uint32_t));
-        s = ((EverCrypt_Hash_state_s){ .tag = SHA1_s, { .case_SHA1_s = buf } });
+        s = ((state_s){ .tag = SHA1_s, { .case_SHA1_s = buf } });
         break;
       }
     case Spec_Hash_Definitions_SHA2_224:
       {
         uint32_t *buf = (uint32_t *)KRML_HOST_CALLOC(8U, sizeof (uint32_t));
-        s = ((EverCrypt_Hash_state_s){ .tag = SHA2_224_s, { .case_SHA2_224_s = buf } });
+        s = ((state_s){ .tag = SHA2_224_s, { .case_SHA2_224_s = buf } });
         break;
       }
     case Spec_Hash_Definitions_SHA2_256:
       {
         uint32_t *buf = (uint32_t *)KRML_HOST_CALLOC(8U, sizeof (uint32_t));
-        s = ((EverCrypt_Hash_state_s){ .tag = SHA2_256_s, { .case_SHA2_256_s = buf } });
+        s = ((state_s){ .tag = SHA2_256_s, { .case_SHA2_256_s = buf } });
         break;
       }
     case Spec_Hash_Definitions_SHA2_384:
       {
         uint64_t *buf = (uint64_t *)KRML_HOST_CALLOC(8U, sizeof (uint64_t));
-        s = ((EverCrypt_Hash_state_s){ .tag = SHA2_384_s, { .case_SHA2_384_s = buf } });
+        s = ((state_s){ .tag = SHA2_384_s, { .case_SHA2_384_s = buf } });
         break;
       }
     case Spec_Hash_Definitions_SHA2_512:
       {
         uint64_t *buf = (uint64_t *)KRML_HOST_CALLOC(8U, sizeof (uint64_t));
-        s = ((EverCrypt_Hash_state_s){ .tag = SHA2_512_s, { .case_SHA2_512_s = buf } });
+        s = ((state_s){ .tag = SHA2_512_s, { .case_SHA2_512_s = buf } });
         break;
       }
     case Spec_Hash_Definitions_SHA3_224:
       {
         uint64_t *buf = (uint64_t *)KRML_HOST_CALLOC(25U, sizeof (uint64_t));
-        s = ((EverCrypt_Hash_state_s){ .tag = SHA3_224_s, { .case_SHA3_224_s = buf } });
+        s = ((state_s){ .tag = SHA3_224_s, { .case_SHA3_224_s = buf } });
         break;
       }
     case Spec_Hash_Definitions_SHA3_256:
       {
         uint64_t *buf = (uint64_t *)KRML_HOST_CALLOC(25U, sizeof (uint64_t));
-        s = ((EverCrypt_Hash_state_s){ .tag = SHA3_256_s, { .case_SHA3_256_s = buf } });
+        s = ((state_s){ .tag = SHA3_256_s, { .case_SHA3_256_s = buf } });
         break;
       }
     case Spec_Hash_Definitions_SHA3_384:
       {
         uint64_t *buf = (uint64_t *)KRML_HOST_CALLOC(25U, sizeof (uint64_t));
-        s = ((EverCrypt_Hash_state_s){ .tag = SHA3_384_s, { .case_SHA3_384_s = buf } });
+        s = ((state_s){ .tag = SHA3_384_s, { .case_SHA3_384_s = buf } });
         break;
       }
     case Spec_Hash_Definitions_SHA3_512:
       {
         uint64_t *buf = (uint64_t *)KRML_HOST_CALLOC(25U, sizeof (uint64_t));
-        s = ((EverCrypt_Hash_state_s){ .tag = SHA3_512_s, { .case_SHA3_512_s = buf } });
+        s = ((state_s){ .tag = SHA3_512_s, { .case_SHA3_512_s = buf } });
         break;
       }
     case Spec_Hash_Definitions_Blake2S:
@@ -216,7 +216,7 @@ static EverCrypt_Hash_state_s *create_in(Spec_Hash_Definitions_hash_alg a)
         {
           s =
             (
-              (EverCrypt_Hash_state_s){
+              (state_s){
                 .tag = Blake2S_128_s,
                 { .case_Blake2S_128_s = Hacl_Hash_Blake2s_Simd128_malloc_with_key() }
               }
@@ -225,11 +225,11 @@ static EverCrypt_Hash_state_s *create_in(Spec_Hash_Definitions_hash_alg a)
         else
         {
           uint32_t *buf = (uint32_t *)KRML_HOST_CALLOC(16U, sizeof (uint32_t));
-          s = ((EverCrypt_Hash_state_s){ .tag = Blake2S_s, { .case_Blake2S_s = buf } });
+          s = ((state_s){ .tag = Blake2S_s, { .case_Blake2S_s = buf } });
         }
         #else
         uint32_t *buf = (uint32_t *)KRML_HOST_CALLOC(16U, sizeof (uint32_t));
-        s = ((EverCrypt_Hash_state_s){ .tag = Blake2S_s, { .case_Blake2S_s = buf } });
+        s = ((state_s){ .tag = Blake2S_s, { .case_Blake2S_s = buf } });
         #endif
         break;
       }
@@ -241,7 +241,7 @@ static EverCrypt_Hash_state_s *create_in(Spec_Hash_Definitions_hash_alg a)
         {
           s =
             (
-              (EverCrypt_Hash_state_s){
+              (state_s){
                 .tag = Blake2B_256_s,
                 { .case_Blake2B_256_s = Hacl_Hash_Blake2b_Simd256_malloc_with_key() }
               }
@@ -250,11 +250,11 @@ static EverCrypt_Hash_state_s *create_in(Spec_Hash_Definitions_hash_alg a)
         else
         {
           uint64_t *buf = (uint64_t *)KRML_HOST_CALLOC(16U, sizeof (uint64_t));
-          s = ((EverCrypt_Hash_state_s){ .tag = Blake2B_s, { .case_Blake2B_s = buf } });
+          s = ((state_s){ .tag = Blake2B_s, { .case_Blake2B_s = buf } });
         }
         #else
         uint64_t *buf = (uint64_t *)KRML_HOST_CALLOC(16U, sizeof (uint64_t));
-        s = ((EverCrypt_Hash_state_s){ .tag = Blake2B_s, { .case_Blake2B_s = buf } });
+        s = ((state_s){ .tag = Blake2B_s, { .case_Blake2B_s = buf } });
         #endif
         break;
       }
@@ -264,15 +264,14 @@ static EverCrypt_Hash_state_s *create_in(Spec_Hash_Definitions_hash_alg a)
         KRML_HOST_EXIT(253U);
       }
   }
-  EverCrypt_Hash_state_s
-  *buf = (EverCrypt_Hash_state_s *)KRML_HOST_MALLOC(sizeof (EverCrypt_Hash_state_s));
+  state_s *buf = (state_s *)KRML_HOST_MALLOC(sizeof (state_s));
   buf[0U] = s;
   return buf;
 }
 
-static void init(EverCrypt_Hash_state_s *s)
+static void init(state_s *s)
 {
-  EverCrypt_Hash_state_s scrut = *s;
+  state_s scrut = *s;
   if (scrut.tag == MD5_s)
   {
     uint32_t *p1 = scrut.case_MD5_s;
@@ -407,10 +406,9 @@ void EverCrypt_Hash_update_multi_256(uint32_t *s, uint8_t *blocks, uint32_t n)
   #endif
 }
 
-static void
-update_multi(EverCrypt_Hash_state_s *s, uint64_t prevlen, uint8_t *blocks, uint32_t len)
+static void update_multi(state_s *s, uint64_t prevlen, uint8_t *blocks, uint32_t len)
 {
-  EverCrypt_Hash_state_s scrut = *s;
+  state_s scrut = *s;
   if (scrut.tag == MD5_s)
   {
     uint32_t *p1 = scrut.case_MD5_s;
@@ -540,10 +538,9 @@ update_multi(EverCrypt_Hash_state_s *s, uint64_t prevlen, uint8_t *blocks, uint3
   KRML_HOST_EXIT(255U);
 }
 
-static void
-update_last(EverCrypt_Hash_state_s *s, uint64_t prev_len, uint8_t *last, uint32_t last_len)
+static void update_last(state_s *s, uint64_t prev_len, uint8_t *last, uint32_t last_len)
 {
-  EverCrypt_Hash_state_s scrut = *s;
+  state_s scrut = *s;
   if (scrut.tag == MD5_s)
   {
     uint32_t *p1 = scrut.case_MD5_s;
@@ -667,9 +664,9 @@ update_last(EverCrypt_Hash_state_s *s, uint64_t prev_len, uint8_t *last, uint32_
   KRML_HOST_EXIT(255U);
 }
 
-static void finish(EverCrypt_Hash_state_s *s, uint8_t *dst)
+static void finish(state_s *s, uint8_t *dst)
 {
-  EverCrypt_Hash_state_s scrut = *s;
+  state_s scrut = *s;
   if (scrut.tag == MD5_s)
   {
     uint32_t *p1 = scrut.case_MD5_s;
@@ -771,9 +768,9 @@ static void finish(EverCrypt_Hash_state_s *s, uint8_t *dst)
   KRML_HOST_EXIT(255U);
 }
 
-static void free_(EverCrypt_Hash_state_s *s)
+static void free_(state_s *s)
 {
-  EverCrypt_Hash_state_s scrut = *s;
+  state_s scrut = *s;
   if (scrut.tag == MD5_s)
   {
     uint32_t *p1 = scrut.case_MD5_s;
@@ -855,13 +852,13 @@ static void free_(EverCrypt_Hash_state_s *s)
   KRML_HOST_FREE(s);
 }
 
-static void copy(EverCrypt_Hash_state_s *s_src, EverCrypt_Hash_state_s *s_dst)
+static void copy(state_s *s_src, state_s *s_dst)
 {
-  EverCrypt_Hash_state_s scrut0 = *s_src;
+  state_s scrut0 = *s_src;
   if (scrut0.tag == MD5_s)
   {
     uint32_t *p_src = scrut0.case_MD5_s;
-    EverCrypt_Hash_state_s x1 = *s_dst;
+    state_s x1 = *s_dst;
     uint32_t *p_dst;
     if (x1.tag == MD5_s)
     {
@@ -877,7 +874,7 @@ static void copy(EverCrypt_Hash_state_s *s_src, EverCrypt_Hash_state_s *s_dst)
   if (scrut0.tag == SHA1_s)
   {
     uint32_t *p_src = scrut0.case_SHA1_s;
-    EverCrypt_Hash_state_s x1 = *s_dst;
+    state_s x1 = *s_dst;
     uint32_t *p_dst;
     if (x1.tag == SHA1_s)
     {
@@ -893,7 +890,7 @@ static void copy(EverCrypt_Hash_state_s *s_src, EverCrypt_Hash_state_s *s_dst)
   if (scrut0.tag == SHA2_224_s)
   {
     uint32_t *p_src = scrut0.case_SHA2_224_s;
-    EverCrypt_Hash_state_s x1 = *s_dst;
+    state_s x1 = *s_dst;
     uint32_t *p_dst;
     if (x1.tag == SHA2_224_s)
     {
@@ -909,7 +906,7 @@ static void copy(EverCrypt_Hash_state_s *s_src, EverCrypt_Hash_state_s *s_dst)
   if (scrut0.tag == SHA2_256_s)
   {
     uint32_t *p_src = scrut0.case_SHA2_256_s;
-    EverCrypt_Hash_state_s x1 = *s_dst;
+    state_s x1 = *s_dst;
     uint32_t *p_dst;
     if (x1.tag == SHA2_256_s)
     {
@@ -925,7 +922,7 @@ static void copy(EverCrypt_Hash_state_s *s_src, EverCrypt_Hash_state_s *s_dst)
   if (scrut0.tag == SHA2_384_s)
   {
     uint64_t *p_src = scrut0.case_SHA2_384_s;
-    EverCrypt_Hash_state_s x1 = *s_dst;
+    state_s x1 = *s_dst;
     uint64_t *p_dst;
     if (x1.tag == SHA2_384_s)
     {
@@ -941,7 +938,7 @@ static void copy(EverCrypt_Hash_state_s *s_src, EverCrypt_Hash_state_s *s_dst)
   if (scrut0.tag == SHA2_512_s)
   {
     uint64_t *p_src = scrut0.case_SHA2_512_s;
-    EverCrypt_Hash_state_s x1 = *s_dst;
+    state_s x1 = *s_dst;
     uint64_t *p_dst;
     if (x1.tag == SHA2_512_s)
     {
@@ -957,7 +954,7 @@ static void copy(EverCrypt_Hash_state_s *s_src, EverCrypt_Hash_state_s *s_dst)
   if (scrut0.tag == SHA3_224_s)
   {
     uint64_t *p_src = scrut0.case_SHA3_224_s;
-    EverCrypt_Hash_state_s x1 = *s_dst;
+    state_s x1 = *s_dst;
     uint64_t *p_dst;
     if (x1.tag == SHA3_224_s)
     {
@@ -973,7 +970,7 @@ static void copy(EverCrypt_Hash_state_s *s_src, EverCrypt_Hash_state_s *s_dst)
   if (scrut0.tag == SHA3_256_s)
   {
     uint64_t *p_src = scrut0.case_SHA3_256_s;
-    EverCrypt_Hash_state_s x1 = *s_dst;
+    state_s x1 = *s_dst;
     uint64_t *p_dst;
     if (x1.tag == SHA3_256_s)
     {
@@ -989,7 +986,7 @@ static void copy(EverCrypt_Hash_state_s *s_src, EverCrypt_Hash_state_s *s_dst)
   if (scrut0.tag == SHA3_384_s)
   {
     uint64_t *p_src = scrut0.case_SHA3_384_s;
-    EverCrypt_Hash_state_s x1 = *s_dst;
+    state_s x1 = *s_dst;
     uint64_t *p_dst;
     if (x1.tag == SHA3_384_s)
     {
@@ -1005,7 +1002,7 @@ static void copy(EverCrypt_Hash_state_s *s_src, EverCrypt_Hash_state_s *s_dst)
   if (scrut0.tag == SHA3_512_s)
   {
     uint64_t *p_src = scrut0.case_SHA3_512_s;
-    EverCrypt_Hash_state_s x1 = *s_dst;
+    state_s x1 = *s_dst;
     uint64_t *p_dst;
     if (x1.tag == SHA3_512_s)
     {
@@ -1021,7 +1018,7 @@ static void copy(EverCrypt_Hash_state_s *s_src, EverCrypt_Hash_state_s *s_dst)
   if (scrut0.tag == Blake2S_s)
   {
     uint32_t *p_src = scrut0.case_Blake2S_s;
-    EverCrypt_Hash_state_s scrut = *s_dst;
+    state_s scrut = *s_dst;
     if (scrut.tag == Blake2S_s)
     {
       uint32_t *p_dst = scrut.case_Blake2S_s;
@@ -1048,7 +1045,7 @@ static void copy(EverCrypt_Hash_state_s *s_src, EverCrypt_Hash_state_s *s_dst)
   if (scrut0.tag == Blake2B_s)
   {
     uint64_t *p_src = scrut0.case_Blake2B_s;
-    EverCrypt_Hash_state_s scrut = *s_dst;
+    state_s scrut = *s_dst;
     if (scrut.tag == Blake2B_s)
     {
       uint64_t *p_dst = scrut.case_Blake2B_s;
@@ -1075,7 +1072,7 @@ static void copy(EverCrypt_Hash_state_s *s_src, EverCrypt_Hash_state_s *s_dst)
   if (scrut0.tag == Blake2S_128_s)
   {
     Lib_IntVector_Intrinsics_vec128 *p_src = scrut0.case_Blake2S_128_s;
-    EverCrypt_Hash_state_s scrut = *s_dst;
+    state_s scrut = *s_dst;
     if (scrut.tag == Blake2S_128_s)
     {
       Lib_IntVector_Intrinsics_vec128 *p_dst = scrut.case_Blake2S_128_s;
@@ -1102,7 +1099,7 @@ static void copy(EverCrypt_Hash_state_s *s_src, EverCrypt_Hash_state_s *s_dst)
   if (scrut0.tag == Blake2B_256_s)
   {
     Lib_IntVector_Intrinsics_vec256 *p_src = scrut0.case_Blake2B_256_s;
-    EverCrypt_Hash_state_s scrut = *s_dst;
+    state_s scrut = *s_dst;
     if (scrut.tag == Blake2B_256_s)
     {
       Lib_IntVector_Intrinsics_vec256 *p_dst = scrut.case_Blake2B_256_s;
@@ -1261,6 +1258,14 @@ static uint32_t block_len(Spec_Hash_Definitions_hash_alg a)
   }
 }
 
+typedef struct EverCrypt_Hash_Incremental_state_t_s
+{
+  state_s *block_state;
+  uint8_t *buf;
+  uint64_t total_len;
+}
+EverCrypt_Hash_Incremental_state_t;
+
 /**
 Allocate initial state for the agile hash. The argument `a` stands for the
 choice of algorithm (see Hacl_Spec.h). This API will automatically pick the most
@@ -1272,7 +1277,7 @@ EverCrypt_Hash_Incremental_state_t
 {
   KRML_CHECK_SIZE(sizeof (uint8_t), block_len(a));
   uint8_t *buf = (uint8_t *)KRML_HOST_CALLOC(block_len(a), sizeof (uint8_t));
-  EverCrypt_Hash_state_s *block_state = create_in(a);
+  state_s *block_state = create_in(a);
   EverCrypt_Hash_Incremental_state_t
   s = { .block_state = block_state, .buf = buf, .total_len = (uint64_t)0U };
   EverCrypt_Hash_Incremental_state_t
@@ -1292,7 +1297,7 @@ void EverCrypt_Hash_Incremental_reset(EverCrypt_Hash_Incremental_state_t *state)
 {
   EverCrypt_Hash_Incremental_state_t scrut = *state;
   uint8_t *buf = scrut.buf;
-  EverCrypt_Hash_state_s *block_state = scrut.block_state;
+  state_s *block_state = scrut.block_state;
   Spec_Hash_Definitions_hash_alg i = alg_of_state(block_state);
   KRML_MAYBE_UNUSED_VAR(i);
   init(block_state);
@@ -1316,7 +1321,7 @@ EverCrypt_Hash_Incremental_update(
 )
 {
   EverCrypt_Hash_Incremental_state_t s = *state;
-  EverCrypt_Hash_state_s *block_state = s.block_state;
+  state_s *block_state = s.block_state;
   uint64_t total_len = s.total_len;
   Spec_Hash_Definitions_hash_alg i1 = alg_of_state(block_state);
   uint64_t sw;
@@ -1417,7 +1422,7 @@ EverCrypt_Hash_Incremental_update(
     if (chunk_len <= block_len(i1) - sz)
     {
       EverCrypt_Hash_Incremental_state_t s1 = *state;
-      EverCrypt_Hash_state_s *block_state1 = s1.block_state;
+      state_s *block_state1 = s1.block_state;
       uint8_t *buf = s1.buf;
       uint64_t total_len1 = s1.total_len;
       uint32_t sz1;
@@ -1445,7 +1450,7 @@ EverCrypt_Hash_Incremental_update(
     else if (sz == 0U)
     {
       EverCrypt_Hash_Incremental_state_t s1 = *state;
-      EverCrypt_Hash_state_s *block_state1 = s1.block_state;
+      state_s *block_state1 = s1.block_state;
       uint8_t *buf = s1.buf;
       uint64_t total_len1 = s1.total_len;
       uint32_t sz1;
@@ -1495,7 +1500,7 @@ EverCrypt_Hash_Incremental_update(
       uint8_t *chunk1 = chunk;
       uint8_t *chunk2 = chunk + diff;
       EverCrypt_Hash_Incremental_state_t s1 = *state;
-      EverCrypt_Hash_state_s *block_state10 = s1.block_state;
+      state_s *block_state10 = s1.block_state;
       uint8_t *buf0 = s1.buf;
       uint64_t total_len10 = s1.total_len;
       uint32_t sz10;
@@ -1520,7 +1525,7 @@ EverCrypt_Hash_Incremental_update(
           }
         );
       EverCrypt_Hash_Incremental_state_t s10 = *state;
-      EverCrypt_Hash_state_s *block_state1 = s10.block_state;
+      state_s *block_state1 = s10.block_state;
       uint8_t *buf = s10.buf;
       uint64_t total_len1 = s10.total_len;
       uint32_t sz1;
@@ -1593,7 +1598,7 @@ EverCrypt_Hash_Incremental_update(
 static void digest_md5(EverCrypt_Hash_Incremental_state_t *state, uint8_t *output)
 {
   EverCrypt_Hash_Incremental_state_t scrut = *state;
-  EverCrypt_Hash_state_s *block_state = scrut.block_state;
+  state_s *block_state = scrut.block_state;
   uint8_t *buf_ = scrut.buf;
   uint64_t total_len = scrut.total_len;
   uint32_t r;
@@ -1607,8 +1612,8 @@ static void digest_md5(EverCrypt_Hash_Incremental_state_t *state, uint8_t *outpu
   }
   uint8_t *buf_1 = buf_;
   uint32_t buf[4U] = { 0U };
-  EverCrypt_Hash_state_s s = { .tag = MD5_s, { .case_MD5_s = buf } };
-  EverCrypt_Hash_state_s tmp_block_state = s;
+  state_s s = { .tag = MD5_s, { .case_MD5_s = buf } };
+  state_s tmp_block_state = s;
   copy(block_state, &tmp_block_state);
   uint64_t prev_len = total_len - (uint64_t)r;
   uint32_t ite;
@@ -1631,7 +1636,7 @@ static void digest_md5(EverCrypt_Hash_Incremental_state_t *state, uint8_t *outpu
 static void digest_sha1(EverCrypt_Hash_Incremental_state_t *state, uint8_t *output)
 {
   EverCrypt_Hash_Incremental_state_t scrut = *state;
-  EverCrypt_Hash_state_s *block_state = scrut.block_state;
+  state_s *block_state = scrut.block_state;
   uint8_t *buf_ = scrut.buf;
   uint64_t total_len = scrut.total_len;
   uint32_t r;
@@ -1645,8 +1650,8 @@ static void digest_sha1(EverCrypt_Hash_Incremental_state_t *state, uint8_t *outp
   }
   uint8_t *buf_1 = buf_;
   uint32_t buf[5U] = { 0U };
-  EverCrypt_Hash_state_s s = { .tag = SHA1_s, { .case_SHA1_s = buf } };
-  EverCrypt_Hash_state_s tmp_block_state = s;
+  state_s s = { .tag = SHA1_s, { .case_SHA1_s = buf } };
+  state_s tmp_block_state = s;
   copy(block_state, &tmp_block_state);
   uint64_t prev_len = total_len - (uint64_t)r;
   uint32_t ite;
@@ -1669,7 +1674,7 @@ static void digest_sha1(EverCrypt_Hash_Incremental_state_t *state, uint8_t *outp
 static void digest_sha224(EverCrypt_Hash_Incremental_state_t *state, uint8_t *output)
 {
   EverCrypt_Hash_Incremental_state_t scrut = *state;
-  EverCrypt_Hash_state_s *block_state = scrut.block_state;
+  state_s *block_state = scrut.block_state;
   uint8_t *buf_ = scrut.buf;
   uint64_t total_len = scrut.total_len;
   uint32_t r;
@@ -1684,8 +1689,8 @@ static void digest_sha224(EverCrypt_Hash_Incremental_state_t *state, uint8_t *ou
   }
   uint8_t *buf_1 = buf_;
   uint32_t buf[8U] = { 0U };
-  EverCrypt_Hash_state_s s = { .tag = SHA2_224_s, { .case_SHA2_224_s = buf } };
-  EverCrypt_Hash_state_s tmp_block_state = s;
+  state_s s = { .tag = SHA2_224_s, { .case_SHA2_224_s = buf } };
+  state_s tmp_block_state = s;
   copy(block_state, &tmp_block_state);
   uint64_t prev_len = total_len - (uint64_t)r;
   uint32_t ite;
@@ -1708,7 +1713,7 @@ static void digest_sha224(EverCrypt_Hash_Incremental_state_t *state, uint8_t *ou
 static void digest_sha256(EverCrypt_Hash_Incremental_state_t *state, uint8_t *output)
 {
   EverCrypt_Hash_Incremental_state_t scrut = *state;
-  EverCrypt_Hash_state_s *block_state = scrut.block_state;
+  state_s *block_state = scrut.block_state;
   uint8_t *buf_ = scrut.buf;
   uint64_t total_len = scrut.total_len;
   uint32_t r;
@@ -1723,8 +1728,8 @@ static void digest_sha256(EverCrypt_Hash_Incremental_state_t *state, uint8_t *ou
   }
   uint8_t *buf_1 = buf_;
   uint32_t buf[8U] = { 0U };
-  EverCrypt_Hash_state_s s = { .tag = SHA2_256_s, { .case_SHA2_256_s = buf } };
-  EverCrypt_Hash_state_s tmp_block_state = s;
+  state_s s = { .tag = SHA2_256_s, { .case_SHA2_256_s = buf } };
+  state_s tmp_block_state = s;
   copy(block_state, &tmp_block_state);
   uint64_t prev_len = total_len - (uint64_t)r;
   uint32_t ite;
@@ -1747,7 +1752,7 @@ static void digest_sha256(EverCrypt_Hash_Incremental_state_t *state, uint8_t *ou
 static void digest_sha3_224(EverCrypt_Hash_Incremental_state_t *state, uint8_t *output)
 {
   EverCrypt_Hash_Incremental_state_t scrut = *state;
-  EverCrypt_Hash_state_s *block_state = scrut.block_state;
+  state_s *block_state = scrut.block_state;
   uint8_t *buf_ = scrut.buf;
   uint64_t total_len = scrut.total_len;
   uint32_t r;
@@ -1762,8 +1767,8 @@ static void digest_sha3_224(EverCrypt_Hash_Incremental_state_t *state, uint8_t *
   }
   uint8_t *buf_1 = buf_;
   uint64_t buf[25U] = { 0U };
-  EverCrypt_Hash_state_s s = { .tag = SHA3_224_s, { .case_SHA3_224_s = buf } };
-  EverCrypt_Hash_state_s tmp_block_state = s;
+  state_s s = { .tag = SHA3_224_s, { .case_SHA3_224_s = buf } };
+  state_s tmp_block_state = s;
   copy(block_state, &tmp_block_state);
   uint64_t prev_len = total_len - (uint64_t)r;
   uint32_t ite;
@@ -1786,7 +1791,7 @@ static void digest_sha3_224(EverCrypt_Hash_Incremental_state_t *state, uint8_t *
 static void digest_sha3_256(EverCrypt_Hash_Incremental_state_t *state, uint8_t *output)
 {
   EverCrypt_Hash_Incremental_state_t scrut = *state;
-  EverCrypt_Hash_state_s *block_state = scrut.block_state;
+  state_s *block_state = scrut.block_state;
   uint8_t *buf_ = scrut.buf;
   uint64_t total_len = scrut.total_len;
   uint32_t r;
@@ -1801,8 +1806,8 @@ static void digest_sha3_256(EverCrypt_Hash_Incremental_state_t *state, uint8_t *
   }
   uint8_t *buf_1 = buf_;
   uint64_t buf[25U] = { 0U };
-  EverCrypt_Hash_state_s s = { .tag = SHA3_256_s, { .case_SHA3_256_s = buf } };
-  EverCrypt_Hash_state_s tmp_block_state = s;
+  state_s s = { .tag = SHA3_256_s, { .case_SHA3_256_s = buf } };
+  state_s tmp_block_state = s;
   copy(block_state, &tmp_block_state);
   uint64_t prev_len = total_len - (uint64_t)r;
   uint32_t ite;
@@ -1825,7 +1830,7 @@ static void digest_sha3_256(EverCrypt_Hash_Incremental_state_t *state, uint8_t *
 static void digest_sha3_384(EverCrypt_Hash_Incremental_state_t *state, uint8_t *output)
 {
   EverCrypt_Hash_Incremental_state_t scrut = *state;
-  EverCrypt_Hash_state_s *block_state = scrut.block_state;
+  state_s *block_state = scrut.block_state;
   uint8_t *buf_ = scrut.buf;
   uint64_t total_len = scrut.total_len;
   uint32_t r;
@@ -1840,8 +1845,8 @@ static void digest_sha3_384(EverCrypt_Hash_Incremental_state_t *state, uint8_t *
   }
   uint8_t *buf_1 = buf_;
   uint64_t buf[25U] = { 0U };
-  EverCrypt_Hash_state_s s = { .tag = SHA3_384_s, { .case_SHA3_384_s = buf } };
-  EverCrypt_Hash_state_s tmp_block_state = s;
+  state_s s = { .tag = SHA3_384_s, { .case_SHA3_384_s = buf } };
+  state_s tmp_block_state = s;
   copy(block_state, &tmp_block_state);
   uint64_t prev_len = total_len - (uint64_t)r;
   uint32_t ite;
@@ -1864,7 +1869,7 @@ static void digest_sha3_384(EverCrypt_Hash_Incremental_state_t *state, uint8_t *
 static void digest_sha3_512(EverCrypt_Hash_Incremental_state_t *state, uint8_t *output)
 {
   EverCrypt_Hash_Incremental_state_t scrut = *state;
-  EverCrypt_Hash_state_s *block_state = scrut.block_state;
+  state_s *block_state = scrut.block_state;
   uint8_t *buf_ = scrut.buf;
   uint64_t total_len = scrut.total_len;
   uint32_t r;
@@ -1879,8 +1884,8 @@ static void digest_sha3_512(EverCrypt_Hash_Incremental_state_t *state, uint8_t *
   }
   uint8_t *buf_1 = buf_;
   uint64_t buf[25U] = { 0U };
-  EverCrypt_Hash_state_s s = { .tag = SHA3_512_s, { .case_SHA3_512_s = buf } };
-  EverCrypt_Hash_state_s tmp_block_state = s;
+  state_s s = { .tag = SHA3_512_s, { .case_SHA3_512_s = buf } };
+  state_s tmp_block_state = s;
   copy(block_state, &tmp_block_state);
   uint64_t prev_len = total_len - (uint64_t)r;
   uint32_t ite;
@@ -1903,7 +1908,7 @@ static void digest_sha3_512(EverCrypt_Hash_Incremental_state_t *state, uint8_t *
 static void digest_sha384(EverCrypt_Hash_Incremental_state_t *state, uint8_t *output)
 {
   EverCrypt_Hash_Incremental_state_t scrut = *state;
-  EverCrypt_Hash_state_s *block_state = scrut.block_state;
+  state_s *block_state = scrut.block_state;
   uint8_t *buf_ = scrut.buf;
   uint64_t total_len = scrut.total_len;
   uint32_t r;
@@ -1918,8 +1923,8 @@ static void digest_sha384(EverCrypt_Hash_Incremental_state_t *state, uint8_t *ou
   }
   uint8_t *buf_1 = buf_;
   uint64_t buf[8U] = { 0U };
-  EverCrypt_Hash_state_s s = { .tag = SHA2_384_s, { .case_SHA2_384_s = buf } };
-  EverCrypt_Hash_state_s tmp_block_state = s;
+  state_s s = { .tag = SHA2_384_s, { .case_SHA2_384_s = buf } };
+  state_s tmp_block_state = s;
   copy(block_state, &tmp_block_state);
   uint64_t prev_len = total_len - (uint64_t)r;
   uint32_t ite;
@@ -1942,7 +1947,7 @@ static void digest_sha384(EverCrypt_Hash_Incremental_state_t *state, uint8_t *ou
 static void digest_sha512(EverCrypt_Hash_Incremental_state_t *state, uint8_t *output)
 {
   EverCrypt_Hash_Incremental_state_t scrut = *state;
-  EverCrypt_Hash_state_s *block_state = scrut.block_state;
+  state_s *block_state = scrut.block_state;
   uint8_t *buf_ = scrut.buf;
   uint64_t total_len = scrut.total_len;
   uint32_t r;
@@ -1957,8 +1962,8 @@ static void digest_sha512(EverCrypt_Hash_Incremental_state_t *state, uint8_t *ou
   }
   uint8_t *buf_1 = buf_;
   uint64_t buf[8U] = { 0U };
-  EverCrypt_Hash_state_s s = { .tag = SHA2_512_s, { .case_SHA2_512_s = buf } };
-  EverCrypt_Hash_state_s tmp_block_state = s;
+  state_s s = { .tag = SHA2_512_s, { .case_SHA2_512_s = buf } };
+  state_s tmp_block_state = s;
   copy(block_state, &tmp_block_state);
   uint64_t prev_len = total_len - (uint64_t)r;
   uint32_t ite;
@@ -1981,7 +1986,7 @@ static void digest_sha512(EverCrypt_Hash_Incremental_state_t *state, uint8_t *ou
 static void digest_blake2s(EverCrypt_Hash_Incremental_state_t *state, uint8_t *output)
 {
   EverCrypt_Hash_Incremental_state_t scrut = *state;
-  EverCrypt_Hash_state_s *block_state = scrut.block_state;
+  state_s *block_state = scrut.block_state;
   uint8_t *buf_ = scrut.buf;
   uint64_t total_len = scrut.total_len;
   uint32_t r;
@@ -1994,24 +1999,24 @@ static void digest_blake2s(EverCrypt_Hash_Incremental_state_t *state, uint8_t *o
     r = (uint32_t)(total_len % (uint64_t)block_len(Spec_Hash_Definitions_Blake2S));
   }
   uint8_t *buf_1 = buf_;
-  EverCrypt_Hash_state_s s;
+  state_s s;
   #if HACL_CAN_COMPILE_VEC128
   bool vec128 = EverCrypt_AutoConfig2_has_vec128();
   KRML_PRE_ALIGN(16) Lib_IntVector_Intrinsics_vec128 buf0[4U] KRML_POST_ALIGN(16) = { 0U };
   uint32_t buf[16U] = { 0U };
   if (vec128)
   {
-    s = ((EverCrypt_Hash_state_s){ .tag = Blake2S_128_s, { .case_Blake2S_128_s = buf0 } });
+    s = ((state_s){ .tag = Blake2S_128_s, { .case_Blake2S_128_s = buf0 } });
   }
   else
   {
-    s = ((EverCrypt_Hash_state_s){ .tag = Blake2S_s, { .case_Blake2S_s = buf } });
+    s = ((state_s){ .tag = Blake2S_s, { .case_Blake2S_s = buf } });
   }
   #else
   uint32_t buf[16U] = { 0U };
-  s = ((EverCrypt_Hash_state_s){ .tag = Blake2S_s, { .case_Blake2S_s = buf } });
+  s = ((state_s){ .tag = Blake2S_s, { .case_Blake2S_s = buf } });
   #endif
-  EverCrypt_Hash_state_s tmp_block_state = s;
+  state_s tmp_block_state = s;
   copy(block_state, &tmp_block_state);
   uint64_t prev_len = total_len - (uint64_t)r;
   uint32_t ite;
@@ -2034,7 +2039,7 @@ static void digest_blake2s(EverCrypt_Hash_Incremental_state_t *state, uint8_t *o
 static void digest_blake2b(EverCrypt_Hash_Incremental_state_t *state, uint8_t *output)
 {
   EverCrypt_Hash_Incremental_state_t scrut = *state;
-  EverCrypt_Hash_state_s *block_state = scrut.block_state;
+  state_s *block_state = scrut.block_state;
   uint8_t *buf_ = scrut.buf;
   uint64_t total_len = scrut.total_len;
   uint32_t r;
@@ -2047,24 +2052,24 @@ static void digest_blake2b(EverCrypt_Hash_Incremental_state_t *state, uint8_t *o
     r = (uint32_t)(total_len % (uint64_t)block_len(Spec_Hash_Definitions_Blake2B));
   }
   uint8_t *buf_1 = buf_;
-  EverCrypt_Hash_state_s s;
+  state_s s;
   #if HACL_CAN_COMPILE_VEC256
   bool vec256 = EverCrypt_AutoConfig2_has_vec256();
   KRML_PRE_ALIGN(32) Lib_IntVector_Intrinsics_vec256 buf0[4U] KRML_POST_ALIGN(32) = { 0U };
   uint64_t buf[16U] = { 0U };
   if (vec256)
   {
-    s = ((EverCrypt_Hash_state_s){ .tag = Blake2B_256_s, { .case_Blake2B_256_s = buf0 } });
+    s = ((state_s){ .tag = Blake2B_256_s, { .case_Blake2B_256_s = buf0 } });
   }
   else
   {
-    s = ((EverCrypt_Hash_state_s){ .tag = Blake2B_s, { .case_Blake2B_s = buf } });
+    s = ((state_s){ .tag = Blake2B_s, { .case_Blake2B_s = buf } });
   }
   #else
   uint64_t buf[16U] = { 0U };
-  s = ((EverCrypt_Hash_state_s){ .tag = Blake2B_s, { .case_Blake2B_s = buf } });
+  s = ((state_s){ .tag = Blake2B_s, { .case_Blake2B_s = buf } });
   #endif
-  EverCrypt_Hash_state_s tmp_block_state = s;
+  state_s tmp_block_state = s;
   copy(block_state, &tmp_block_state);
   uint64_t prev_len = total_len - (uint64_t)r;
   uint32_t ite;
@@ -2090,7 +2095,7 @@ Perform a run-time test to determine which algorithm was chosen for the given pi
 Spec_Hash_Definitions_hash_alg
 EverCrypt_Hash_Incremental_alg_of_state(EverCrypt_Hash_Incremental_state_t *s)
 {
-  EverCrypt_Hash_state_s *block_state = (*s).block_state;
+  state_s *block_state = (*s).block_state;
   return alg_of_state(block_state);
 }
 
@@ -2183,7 +2188,7 @@ void EverCrypt_Hash_Incremental_free(EverCrypt_Hash_Incremental_state_t *state)
 {
   EverCrypt_Hash_Incremental_state_t scrut = *state;
   uint8_t *buf = scrut.buf;
-  EverCrypt_Hash_state_s *block_state = scrut.block_state;
+  state_s *block_state = scrut.block_state;
   free_(block_state);
   KRML_HOST_FREE(buf);
   KRML_HOST_FREE(state);
