dist/gcc-compatible/Hacl_Hash_Blake2b.h
@@ -53,28 +53,7 @@ typedef struct Hacl_Hash_Blake2b_blake2_params_s
 }
 Hacl_Hash_Blake2b_blake2_params;
 
-typedef struct K____uint64_t___uint64_t__s
-{
-  uint64_t *fst;
-  uint64_t *snd;
-}
-K____uint64_t___uint64_t_;
-
-typedef struct Hacl_Hash_Blake2b_block_state_t_s
-{
-  uint8_t fst;
-  uint8_t snd;
-  K____uint64_t___uint64_t_ thd;
-}
-Hacl_Hash_Blake2b_block_state_t;
-
-typedef struct Hacl_Hash_Blake2b_state_t_s
-{
-  Hacl_Hash_Blake2b_block_state_t block_state;
-  uint8_t *buf;
-  uint64_t total_len;
-}
-Hacl_Hash_Blake2b_state_t;
+typedef struct Hacl_Hash_Blake2b_state_t_s Hacl_Hash_Blake2b_state_t;
 
 /**
  State allocation function when there are parameters and a key. The
