dist/gcc-compatible/Hacl_Streaming_Types.h
@@ -59,21 +59,9 @@ typedef uint8_t Spec_Hash_Definitions_hash_alg;
 
 typedef uint8_t Hacl_Streaming_Types_error_code;
 
-typedef struct Hacl_Streaming_MD_state_32_s
-{
-  uint32_t *block_state;
-  uint8_t *buf;
-  uint64_t total_len;
-}
-Hacl_Streaming_MD_state_32;
+typedef struct Hacl_Streaming_MD_state_32_s Hacl_Streaming_MD_state_32;
 
-typedef struct Hacl_Streaming_MD_state_64_s
-{
-  uint64_t *block_state;
-  uint8_t *buf;
-  uint64_t total_len;
-}
-Hacl_Streaming_MD_state_64;
+typedef struct Hacl_Streaming_MD_state_64_s Hacl_Streaming_MD_state_64;
 
 #if defined(__cplusplus)
 }
