dist/gcc-compatible/internal/Hacl_Hash_Blake2b.h
@@ -38,6 +38,13 @@ extern "C" {
 #include "internal/Hacl_Impl_Blake2_Constants.h"
 #include "../Hacl_Hash_Blake2b.h"
 
+typedef struct Hacl_Hash_Blake2b_index_s
+{
+  uint8_t key_length;
+  uint8_t digest_length;
+}
+Hacl_Hash_Blake2b_index;
+
 void Hacl_Hash_Blake2b_init(uint64_t *hash, uint32_t kk, uint32_t nn);
 
 void
@@ -61,17 +68,6 @@ Hacl_Hash_Blake2b_update_last(
 );
 
 void Hacl_Hash_Blake2b_finish(uint32_t nn, uint8_t *output, uint64_t *hash);
-
-typedef struct K___uint8_t_uint8_t_s
-{
-  uint8_t fst;
-  uint8_t snd;
-}
-K___uint8_t_uint8_t;
-
-uint8_t FStar_Pervasives_Native_fst__uint8_t_uint8_t(K___uint8_t_uint8_t x);
-
-uint8_t FStar_Pervasives_Native_snd__uint8_t_uint8_t(K___uint8_t_uint8_t x);
 
 typedef struct K____Hacl_Impl_Blake2_Core_blake2_params___uint8_t__s
 {
