dist/gcc-compatible/lib/Hacl_Hash_Blake2b_bindings.ml
@@ -31,45 +31,41 @@ module Bindings(F:Cstubs.FOREIGN) =
     let hacl_Hash_Blake2b_blake2_params_personal =
       field hacl_Hash_Blake2b_blake2_params "personal" (ptr uint8_t)
     let _ = seal hacl_Hash_Blake2b_blake2_params
+    type hacl_Hash_Blake2b_index = [ `hacl_Hash_Blake2b_index ] structure
+    let (hacl_Hash_Blake2b_index :
+      [ `hacl_Hash_Blake2b_index ] structure typ) =
+      structure "Hacl_Hash_Blake2b_index_s"
+    let hacl_Hash_Blake2b_index_key_length =
+      field hacl_Hash_Blake2b_index "key_length" uint8_t
+    let hacl_Hash_Blake2b_index_digest_length =
+      field hacl_Hash_Blake2b_index "digest_length" uint8_t
+    let _ = seal hacl_Hash_Blake2b_index
     let hacl_Hash_Blake2b_init =
       foreign "Hacl_Hash_Blake2b_init"
         ((ptr uint64_t) @-> (uint32_t @-> (uint32_t @-> (returning void))))
     let hacl_Hash_Blake2b_finish =
       foreign "Hacl_Hash_Blake2b_finish"
         (uint32_t @-> (ocaml_bytes @-> ((ptr uint64_t) @-> (returning void))))
-    type k____uint64_t___uint64_t_ = [ `k____uint64_t___uint64_t_ ] structure
-    let (k____uint64_t___uint64_t_ :
-      [ `k____uint64_t___uint64_t_ ] structure typ) =
+    type ___uint64_t___uint64_t_ = [ `___uint64_t___uint64_t_ ] structure
+    let (___uint64_t___uint64_t_ :
+      [ `___uint64_t___uint64_t_ ] structure typ) =
       structure "K____uint64_t___uint64_t__s"
-    let k____uint64_t___uint64_t__fst =
-      field k____uint64_t___uint64_t_ "fst" (ptr uint64_t)
-    let k____uint64_t___uint64_t__snd =
-      field k____uint64_t___uint64_t_ "snd" (ptr uint64_t)
-    let _ = seal k____uint64_t___uint64_t_
-    type hacl_Hash_Blake2b_block_state_t =
-      [ `hacl_Hash_Blake2b_block_state_t ] structure
-    let (hacl_Hash_Blake2b_block_state_t :
-      [ `hacl_Hash_Blake2b_block_state_t ] structure typ) =
+    let ___uint64_t___uint64_t__fst =
+      field ___uint64_t___uint64_t_ "fst" (ptr uint64_t)
+    let ___uint64_t___uint64_t__snd =
+      field ___uint64_t___uint64_t_ "snd" (ptr uint64_t)
+    let _ = seal ___uint64_t___uint64_t_
+    type block_state_t = [ `block_state_t ] structure
+    let (block_state_t : [ `block_state_t ] structure typ) =
       structure "Hacl_Hash_Blake2b_block_state_t_s"
-    let hacl_Hash_Blake2b_block_state_t_fst =
-      field hacl_Hash_Blake2b_block_state_t "fst" uint8_t
-    let hacl_Hash_Blake2b_block_state_t_snd =
-      field hacl_Hash_Blake2b_block_state_t "snd" uint8_t
-    let hacl_Hash_Blake2b_block_state_t_thd =
-      field hacl_Hash_Blake2b_block_state_t "thd" k____uint64_t___uint64_t_
-    let _ = seal hacl_Hash_Blake2b_block_state_t
+    let block_state_t_fst = field block_state_t "fst" uint8_t
+    let block_state_t_snd = field block_state_t "snd" uint8_t
+    let block_state_t_thd = field block_state_t "thd" ___uint64_t___uint64_t_
+    let _ = seal block_state_t
     type hacl_Hash_Blake2b_state_t = [ `hacl_Hash_Blake2b_state_t ] structure
     let (hacl_Hash_Blake2b_state_t :
       [ `hacl_Hash_Blake2b_state_t ] structure typ) =
       structure "Hacl_Hash_Blake2b_state_t_s"
-    let hacl_Hash_Blake2b_state_t_block_state =
-      field hacl_Hash_Blake2b_state_t "block_state"
-        hacl_Hash_Blake2b_block_state_t
-    let hacl_Hash_Blake2b_state_t_buf =
-      field hacl_Hash_Blake2b_state_t "buf" (ptr uint8_t)
-    let hacl_Hash_Blake2b_state_t_total_len =
-      field hacl_Hash_Blake2b_state_t "total_len" uint64_t
-    let _ = seal hacl_Hash_Blake2b_state_t
     let hacl_Hash_Blake2b_malloc_with_params_and_key =
       foreign "Hacl_Hash_Blake2b_malloc_with_params_and_key"
         ((ptr hacl_Hash_Blake2b_blake2_params) @->
