dist/gcc-compatible/lib/Hacl_Hash_Blake2s_Simd128_bindings.ml
@@ -8,6 +8,51 @@ module Bindings(F:Cstubs.FOREIGN) =
     module Hacl_Hash_Blake2b_applied =
       (Hacl_Hash_Blake2b_bindings.Bindings)(Hacl_Hash_Blake2b_stubs)
     open Hacl_Hash_Blake2b_applied
+    type hacl_Hash_Blake2s_Simd128_state_t =
+      [ `hacl_Hash_Blake2s_Simd128_state_t ] structure
+    let (hacl_Hash_Blake2s_Simd128_state_t :
+      [ `hacl_Hash_Blake2s_Simd128_state_t ] structure typ) =
+      structure "Hacl_Hash_Blake2s_Simd128_state_t_s"
+    let hacl_Hash_Blake2s_Simd128_malloc_with_params_and_key =
+      foreign "Hacl_Hash_Blake2s_Simd128_malloc_with_params_and_key"
+        ((ptr hacl_Hash_Blake2b_blake2_params) @->
+           (ocaml_bytes @->
+              (returning (ptr hacl_Hash_Blake2s_Simd128_state_t))))
+    let hacl_Hash_Blake2s_Simd128_malloc_with_key0 =
+      foreign "Hacl_Hash_Blake2s_Simd128_malloc_with_key0"
+        (ocaml_bytes @->
+           (uint8_t @-> (returning (ptr hacl_Hash_Blake2s_Simd128_state_t))))
+    let hacl_Hash_Blake2s_Simd128_malloc =
+      foreign "Hacl_Hash_Blake2s_Simd128_malloc"
+        (void @-> (returning (ptr hacl_Hash_Blake2s_Simd128_state_t)))
+    let hacl_Hash_Blake2s_Simd128_reset_with_key_and_params =
+      foreign "Hacl_Hash_Blake2s_Simd128_reset_with_key_and_params"
+        ((ptr hacl_Hash_Blake2s_Simd128_state_t) @->
+           ((ptr hacl_Hash_Blake2b_blake2_params) @->
+              (ocaml_bytes @-> (returning void))))
+    let hacl_Hash_Blake2s_Simd128_reset_with_key =
+      foreign "Hacl_Hash_Blake2s_Simd128_reset_with_key"
+        ((ptr hacl_Hash_Blake2s_Simd128_state_t) @->
+           (ocaml_bytes @-> (returning void)))
+    let hacl_Hash_Blake2s_Simd128_reset =
+      foreign "Hacl_Hash_Blake2s_Simd128_reset"
+        ((ptr hacl_Hash_Blake2s_Simd128_state_t) @-> (returning void))
+    let hacl_Hash_Blake2s_Simd128_update =
+      foreign "Hacl_Hash_Blake2s_Simd128_update"
+        ((ptr hacl_Hash_Blake2s_Simd128_state_t) @->
+           (ocaml_bytes @->
+              (uint32_t @-> (returning hacl_Streaming_Types_error_code))))
+    let hacl_Hash_Blake2s_Simd128_digest =
+      foreign "Hacl_Hash_Blake2s_Simd128_digest"
+        ((ptr hacl_Hash_Blake2s_Simd128_state_t) @->
+           (ocaml_bytes @-> (returning void)))
+    let hacl_Hash_Blake2s_Simd128_free =
+      foreign "Hacl_Hash_Blake2s_Simd128_free"
+        ((ptr hacl_Hash_Blake2s_Simd128_state_t) @-> (returning void))
+    let hacl_Hash_Blake2s_Simd128_copy =
+      foreign "Hacl_Hash_Blake2s_Simd128_copy"
+        ((ptr hacl_Hash_Blake2s_Simd128_state_t) @->
+           (returning (ptr hacl_Hash_Blake2s_Simd128_state_t)))
     let hacl_Hash_Blake2s_Simd128_hash_with_key =
       foreign "Hacl_Hash_Blake2s_Simd128_hash_with_key"
         (ocaml_bytes @->
